\documentclass[a4paper]{article}
\usepackage[a4paper,top=1.5cm]{geometry}
% \usepackage[a4paper,top=2cm,bottom=2.5cm,left=5cm,right=1.5cm,marginparwidth=1.75cm]{geometry}
\usepackage[utf8]{inputenc}
\usepackage{logicproof}

%% Language and font encodings
\usepackage[english]{babel}
\usepackage[utf8x]{inputenc}
\usepackage{listings}

%% Sets page size and margins

\usepackage{float}
%% Useful packages
\usepackage{amsmath}
\usepackage[colorinlistoftodos]{todonotes}
\usepackage[colorlinks=true, allcolors=blue]{hyperref}
\usepackage{listings}
\usepackage{url}
\usepackage{graphicx}
\graphicspath{ {./images/} }
% \DeclareGraphicsExtensions{.pdf,.jpg,.png}

%% defined colors
\definecolor{Blue}{rgb}{0,0,0.5}
\definecolor{Green}{rgb}{0,0.75,0.0}
\definecolor{LightGray}{rgb}{0.6,0.6,0.6}
\definecolor{DarkGray}{rgb}{0.3,0.3,0.3}


\title{CS540 - Artificial Intelligence: Assignment-1 \\Logic: Forward and Backward Chaining}
% \subtitle{Logic: Forward and Backward Chaining}
\author{Sanket Mehrotra (EID: 832449213) }
\date{February 6, 2021}

\begin{document}

\maketitle

\section{Question:}

\parindent
Given:

$$\lnot(P \to S)$$
$$(P \to A)$$
$$(\lnot B \to S)$$
$$Z \to (\lnot A \land B)$$
$$X \to (\lnot B \land Z)$$
$$(\lnot Z \land \lnot X ) \to Q$$

Prove: $Q$ 


Using : \begin{enumerate}
    \item Forward Chaining
    \item Backward Chaining
\end{enumerate}

\newpage
\section{Forward Chaining}

In forward chaining, we try to use a data driven, Modus Ponens related approach.\\
We first simplify the inferences using logical equivalence into CNF.


{
\setlength\subproofhorizspace{2em}
\begin{logicproof}{1}
    \begin{subproof}
        \lnot(P \to S)  & \\
        \equiv \lnot(\lnot P \lor S) & Implication \\
        \equiv (P \land \lnot S) & DeMorgans
    \end{subproof}
    \begin{subproof}
        $$(P \to A)$$ & \\
        \equiv ( \lnot P \lor A ) & Implication
    \end{subproof}
    \begin{subproof}
        (\lnot B \to S) & \\
        \equiv (B \lor S) & Implication
    \end{subproof}
    \begin{subproof}
        $$Z \to (\lnot A \land B)$$ & \\
        \equiv (\lnot Z \lor \lnot A ) \land ( \lnot Z \lor B ) & Implication
    \end{subproof}
    \begin{subproof}
        $$X \to (\lnot B \land Z)$$ & \\
        \equiv (\lnot X \lor \lnot B) \land (\lnot X \lor Z) & Implication
    \end{subproof}
    \begin{subproof}
        $$(\lnot Z \land \lnot X ) \to Q$$ & \\
        \equiv \lnot Q \to \lnot(\lnot Z \land\lnot X) & Implication\\
        \equiv \lnot Q \to ( Z \lor X) & DeMorgans \\
        \equiv Q \lor Z \lor X & 
    \end{subproof}
    \noindent\rule{4cm}{0.4pt} \\
    P & from 3 \\
    \lnot S & from 3 (Horn Clause Structure)\\
    \lnot P, A & from 5 \\
    B, S & from 7 \\
    \lnot Z, \lnot A & from 9 \\
    \lnot Z, B & from 9 \\
    \lnot X , \lnot B & from 11 \\
    \lnot X, Z & from 11 \\
    Q,Z,X & from 15 \\
    \noindent\rule{4cm}{0.4pt} \\
    \lnot P, \lnot Z & from 19 and 21\\
    B & from 18 and 20 \\
    P, B & from 17 and 28 \\
    P, \lnot X & from 23 and 29 \\
    \lnot Z , \lnot X & from 27 and 30 \\
    Q & from 25 and 31
    
\end{logicproof}
}

\newpage
\section{Backward Chaining}
{
In Backward Chaining, we use a goal driven approach to try to force a fallacy via a proof by contradiction.

In our case we assume that what we are trying to prove: $Q$ is False; i.e. $\lnot Q$ is True.

{
\setlength\subproofhorizspace{2em}
\begin{logicproof}{1}
    \begin{subproof}
        \lnot(P \to S)  & \\
        \equiv \lnot(\lnot P \lor S) & Implication \\
        \equiv (P \land \lnot S) & DeMorgans
    \end{subproof}
    \begin{subproof}
        $$(P \to A)$$ & \\
        \equiv ( \lnot P \lor A ) & Implication
    \end{subproof}
    \begin{subproof}
        (\lnot B \to S) & \\
        \equiv (B \lor S) & Implication
    \end{subproof}
    \begin{subproof}
        $$Z \to (\lnot A \land B)$$ & \\
        \equiv (\lnot Z \lor \lnot A ) \land ( \lnot Z \lor B ) & Implication
    \end{subproof}
    \begin{subproof}
        $$X \to (\lnot B \land Z)$$ & \\
        \equiv (\lnot X \lor \lnot B) \land (\lnot X \lor Z) & Implication
    \end{subproof}
    \begin{subproof}
        $$(\lnot Z \land \lnot X ) \to Q$$ & \\
        \equiv \lnot Q \to \lnot(\lnot Z \land\lnot X) & Implication\\
        \equiv \lnot Q \to ( Z \lor X) & DeMorgans \\
        \equiv Q \lor Z \lor X & 
    \end{subproof}
    % P, \lnot S & from 3 \\
    \noindent\rule{4cm}{0.4pt} \\
    P & from 3 \\
    \lnot S & from 3 (Horn Clause Structure)\\
    \lnot P, A & from 5 \\
    B, S & from 7 \\
    \lnot Z, \lnot A & from 9 \\
    \lnot Z, B & from 9 \\
    \lnot X , \lnot B & from 11 \\
    \lnot X, Z & from 11 \\
    Q,Z,X & from 15 \\
    \noindent\rule{4cm}{0.4pt} \\
    $\lnot Q$ & from assumption\\
    Z, X & from 25 and 27 \\
    B & from 18 and 20 \\
    \lnot X & from 23 and 29 \\
    Z & from 28 and 30 \\
    \lnot Z & from 22 and 29 \\
    % \lnot B & from 30 and 23 \\
    **CONTRADICTION** & 31 and 32
\end{logicproof}
}

}

\end{document}

% {
% \setlength\subproofhorizspace{2em}
% \begin{logicproof}{1}
%     \lnot(P \to S) \equiv \lnot(\lnot P \lor S) \equiv (P \land \lnot S) & Implication Law, DeMorgans Law \\
%     $$(P \to A)$$ \equiv (\lnot P \lor A ) & Implication \\\hspace*{-30pt}
%     \begin{subproof}
%         \llap{$x_0\quad$} P(x_0) \to Q(x_0) & $\forall x \, \mathrm{e}$ 1 \\
%         P(x_0) & $\forall x \, \mathrm{e}$ 2 \\
%         Q(x_0) & $\to \mathrm{e}$ 3, 4
%     \end{subproof}
%     \forall x \, Q(x) & $\forall x \, \mathrm{i}$ 3--5
% \end{logicproof}
% }